\documentclass{ximera}

\input{../../preamble.tex}

\author{Jim Talamo}
\license{Creative Commons 3.0 By-bC}


\outcome{}


\begin{document}
\begin{exercise}
Given that $\sum_{k=5}^{\infty} \frac{8}{k^2-2k} = \frac{7}{3}$, find $\sum_{k=3}^{\infty} \frac{8}{k^2-2k}$.

\[
\sum_{k=3}^{\infty}\frac{8}{k^2-2k} = \answer{6}
\]

\begin{hint}
Write out the given series and relate it to the one we want to find.

\begin{align*}
\sum_{k=5}^{\infty}\frac{8}{k^2-2k}&=\frac{8}{(5)^2-2(5)} + \frac{8}{(6)^2-2(6)} + \ldots \\
\sum_{k=3}^{\infty}\frac{8}{k^2-2k}&= \frac{8}{(3)^2-2(3)} +\frac{8}{(4)^2-2(4)}+\frac{8}{(5)^2-2(5)}+\frac{8}{(6)^2-2(6)}+  \ldots \\
\sum_{k=3}^{\infty}\frac{8}{k^2-2k}&= \frac{8}{(3)^2-2(3)} +\frac{8}{(4)^2-2(4)}+\sum_{k=\answer{5}}^{\infty}\frac{8}{k^2-2k}
\end{align*}
  
Now, use the given information and the above equation to finish the problem.
 \end{hint}

\end{exercise}


\end{document}
