\documentclass{ximera}

\input{../../preamble.tex}

\author{Jim Talamo}
\license{Creative Commons 3.0 By-NC}


\outcome{Evaluate integrals using integration by parts, including mulitple iterations}


\begin{document}
\begin{exercise}
Find the integral $I = \int_0^{\pi} e^{3x}\cos(x) \d x $.

\[
I = \answer{-\frac{3}{10}-\frac{3}{10}e^{3 \pi}}
\]

\begin{hint}
First, set $u = \cos(x)$ and $\d v =  e^{3x}$.  Then, $\d u = \answer{- \sin(x)} \d x$ and $v = \answer{\frac{1}{3}e^{3x}}$.  Applying the integration by parts procedure gives:

\[
I = \eval{\answer{\frac{1}{3}e^{3x}\cos(x)}}_0^{\pi}-\int_0^{\pi} \answer{-\frac{1}{3}e^{3x}\sin(x)} \d x
\] 

and after evaluating the first expression and simplifying, we have:

\[
I = \answer{-\frac{1}{3}e^{3\pi}-\frac{1}{3}}+\int_0^{\pi} \answer{\frac{1}{3}e^{3x}\sin(x)} \d x
\]

\begin{question}
Applying this procedure again, and being consistent with the type of function we use for $u$ and $\d v$ gives:

\begin{align*}
u  &=  \answer{\sin(x)} & \d v &= \frac{1}{3} \answer{e^{3x}} \d x \\
\d u &= \answer{\cos(x)} \d x & v &= \answer{\frac{1}{9} e^{3x}}
\end{align*}

\begin{question}
Applying the integration by parts procedure gives:

\[
I = -\frac{1}{3}e^{3\pi}-\frac{1}{3}+\left(\eval{\answer{\frac{1}{9}e^{3x}\sin(x)}}_0^{\pi} - \int_0^{\pi} \answer{\frac{1}{9} e^{3x}\cos(x)} \d x \right)
\] 

\begin{question}
Simplifying this gives:

\[
I = -\frac{1}{3}e^{3\pi}-\frac{1}{3}- \int_0^{\pi} \answer{\frac{1}{9} e^{3x}\cos(x)} \d x 
\] 

Note that the original integral has appeared again!  We can thus write the above as:

\[
I = -\frac{1}{3}e^{3\pi}-\frac{1}{3}- \answer{\frac{1}{9}} I
\] 

This is an algebraic equation in $I$.  Moving the terms involving $I$ to the lefthand side gives:

\[
\answer{\frac{10}{9}} I = -\frac{1}{3}e^{3\pi}-\frac{1}{3}
\] 

Solve this for $I$ to obtain the value of the original definite integral.


\end{question}
\end{question}
\end{question}
\end{hint}

\end{exercise}
\end{document}
